Finite Differences

Chaang Tze Shen Tristan

January 22, 2022

1 Operators

We define $\Delta f(x) = f(x+1) - f(x)$ as the first order finite difference. The symbol Δ is said to be the finite difference operator. Generally we define

$$\Delta^r f(x) = \Delta(\Delta^{r-1} f(x)) \tag{1}$$

as the r-order finite difference. Also we define the following operators:

1. Ef(x) = f(x+1)

2. If(x) = f(x)

Hence

$$E^{n}f(x) = f(x+n)$$
$$I^{n}f(x) = f(x)$$
$$\Delta = E - I$$

These operations will be very useful in proving some of the propositions below.

2 Finite Differences

Let's start by finding a pattern in finite differences of various orders:

$$\begin{aligned} \Delta^2 f(x) &= f(x+2) - 2f(x+1) + f(x) \\ \Delta^3 f(x) &= f(x+3) - 3f(x+2) + 3f(x+1) - f(x) \\ \Delta^4 f(x) &= f(x+4) - 4f(x+3) + 6f(x+2) - 4f(x+1) + f(x) \end{aligned}$$

As such, we propose the following:

Proposition 1. Let r be a positive integer, then

$$\Delta^{n} f(x) = \sum_{k=0}^{n} (-1)^{k} \binom{n}{k} f(x+n-k)$$
(2)

Proof. Since $\Delta = E - I$,

$$\Delta^n = (E - I)^n = \sum_{k=0}^n (-1)^k \binom{n}{k} E^{n-k} \quad \Box$$

Let's look from a different perspective from Proposition 1, where we write a function in terms of finite differences instead.

$$f(x+1) = \Delta f(x) + f(x)$$

$$f(x+2) = \Delta^2 f(x) + 2\Delta f(x) + f(x)$$

$$f(x+3) = \Delta^3 f(x) + 3\Delta^2 f(x) + 3\Delta f(x) + f(x)$$

Hence we propose the following:

Proposition 2. For any non-negative integer n,

$$f(x+n) = \sum_{k=0}^{n} \binom{n}{k} \Delta^{k} f(x)$$
(3)

Proof. Since $\Delta = E - I$,

$$E^{n} = (\Delta + I)^{n} = \sum_{k=0}^{n} \binom{n}{k} \Delta^{k} \quad \Box$$

Again, this directly brings us to

Proposition 3. For any non-negative integer n,

$$f(n) = \sum_{k=0}^{n} \binom{n}{k} \Delta^{k} f(0)$$

Proof. Proposition 2. x = 0.

We take one step further: Writing $f(1) + \cdots + f(n)$ as a sum of finite differences.

Proposition 4. The sum of the first *n* terms of f(n) is

$$f(1) + \dots + f(n) = \sum_{k=1}^{n} {n \choose k} \Delta^{k-1} f(1)$$
 (4)

Proof. Since $\Delta = E - I$,

$$E^{0} + \dots + E^{n-1} = \frac{E^{n} - I}{E - I} = \frac{(\Delta + I)^{n} - I}{\Delta} = \sum_{k=0}^{n} {n \choose k+1} \Delta^{k} \quad \Box$$

Polynomials 3

Next let's see what happens if we apply finite differences to polynomials:

$$f(x) = a_n x^n + \dots$$

$$\Delta f(x) = n a_n x^{n-1} + \dots$$

$$\Delta^2 f(x) = n(n-1)a_n x^{n-2} + \dots$$

Proposition 5. If f(x) is an *n*-degree polynomial with leading coefficient a_n , then

$$\Delta^n f(x) = n! \cdot a_n \tag{5}$$

Proof. Induct in terms of the leading coefficient.

The following proposition may be very useful and it is very straightforward. We can use it to deal with the degree of a certain polynomial.

Proposition 6. If f(x) is an *n*-degree polynomial, then $\Delta^{n+1}f(x) = 0$ (6)

Proof. From proposition 5 we have $\Delta^{n+1} f(x) = n! \cdot a_n - n! \cdot a_n = 0.$

From proposition 3, we can also generalise n to x, writing f(x) as a sum of what we call finite difference polynomials (which is deep down just a binomial choose function!)

Proposition 7. For any *n*-degree polynomial,

$$f(x) = \sum_{k=0}^{n} \Delta^{k} f(0) \begin{pmatrix} x \\ k \end{pmatrix} \text{ or simply } \sum_{k=0}^{n} c_{k} \begin{pmatrix} x \\ k \end{pmatrix}$$

Proof. $f(x) - \sum_{k=0}^{n} \Delta^{k} f(0) \begin{pmatrix} x \\ k \end{pmatrix} \text{ has } n+1 \text{ roots, hence } 0.$

In fact, the expansion in proposition 7 is unique, and a polynomial is integer valued if and only if $\forall c_i \in \mathbb{Z}$.

Example 1. Let $m \ge n$ be positive integers. Prove that

$$\sum_{k=0}^{n} (-1)^k \binom{m-k}{n} \binom{n}{k} = 1.$$

Solution. Note that $\Delta^n f(x)$ is constant if we let

$$f(x) = \binom{m-x}{n}$$

$$f(x) = \sum_{k=0}^{n} (-1)^{k} \binom{n}{k} f(k)$$

$$= (-1)^{n} \Delta^{n} f(0)$$

$$= (-1)^{n} \Delta^{n} f(m-n)$$

$$= \sum_{k=0}^{n} (-1)^{k} \binom{n}{k} f(m-n+k)$$

$$= 1+0+0+0+\dots = 1 \quad \Box$$

Example 2. Let P(x) be a polynomial of degree n such that

$$P(k) = \binom{n+1}{k}^{-1}$$

for $k = 0, 1, \ldots, n$. Find the value of P(n + 1).

Solution. We start with

$$\Delta^{n+1} P(x) = 0$$

$$\sum_{i=0}^{n+1} (-1)^i \binom{n+1}{i} P(n+1-i) = 0$$

$$P(n+1) + \sum_{i=1}^{n+1} (-1)^i = 0$$

$$\therefore P(n+1) = \begin{cases} 0 & \text{if } n \text{ is even;} \\ 1 & \text{if } n \text{ is odd.} \end{cases}$$

4 Falling Factorials

Let's introduce and define falling factorials.

$$k^{(n)} = k(k-1)\dots(k-n+1).$$

Yes, it is precisely another definition of P_n^k . Take the finite difference

$$\Delta k^{(n)} = (k+1)^{(n)} - k^{(n)}$$

= $(k+1)k^{(n-1)} - k^{(n-1)}(k-n+1)$
= $n \cdot k^{(n-1)}$

and we see it resembles the definition of the derivative! Hence the backward process is analogous, it is called finite integration.

Example 3. Find the value of

$$1^4 + \dots + n^4.$$

Solution.

$$\sum_{k=0}^{n} k^{4} = \sum_{k=0}^{n} (k^{(4)} + 6k^{(3)} + 7k^{(2)} + k^{(1)})$$

= $\sum_{k=0}^{n} \Delta \left(\frac{1}{5}k^{(5)} + \frac{3}{2}k^{(4)} + \frac{7}{3}k^{(3)} + \frac{1}{2}k^{(2)} \right)$
= $\left(\frac{1}{5}(n+1)^{(5)} + \frac{3}{2}(n+1)^{(4)} + \frac{7}{3}(n+1)^{(3)} + \frac{1}{2}(n+1)^{(2)} \right) - 0$
= $\frac{1}{30}n(n+1)(2n+1)(3n^{2} + 3n - 1)$

Example 4. Find the value of

$$2^3 + 5^3 + 8^3 + \dots + (3n+2)^3$$

Solution. We have $f(n) = (3n+2)^3$. Then

$$\sum_{k=0}^{n} (3k+2)^3 = \sum_{k=1}^{n} (27k^{(3)} + 135k^{(2)} + 117k^{(1)} + 8)$$

=
$$\sum_{k=1}^{n} \Delta \left(\frac{27}{4}k^{(4)} + 45k^{(3)} + \frac{117}{2}k^{(2)} + 8k^{(1)} \right)$$

=
$$\frac{27}{4}(n+1)^{(4)} + 45(n+1)^{(3)} + \frac{117}{2}(n+1)^{(2)} + 8(n+1)^{(1)}$$

=
$$\frac{1}{4}(n+1)(3n+4)(9n^2 + 21n + 8)$$

Example 5. Find the value of

$$\sum_{k=0}^{n} (-1)^k \binom{n}{k} k^{n+2}$$

Solution. We basically want $(I - E)^n x^{n+2} = (-1)^n \Delta^n x^{n+2}$ evaluated at x = 0.

$$\Delta^{n}(x^{n+2}) = \Delta^{n} \left(x^{(n+2)} + \left\{ \begin{array}{c} n+2\\ n+1 \end{array} \right\} x^{(n+1)} + \left\{ \begin{array}{c} n+2\\ n \end{array} \right\} x^{(n)} + \cdots \right)$$

so the answer is

$$(-1)^{n} n! \begin{Bmatrix} n+2\\n \end{Bmatrix} = (-1)^{n} n! \cdot \frac{(n+2)(n+1)n(3n+1)}{24} = (-1)^{n} \cdot \frac{(n+2)!(3n+1)n}{24}.$$